\documentclass[main.tex]{subfile}

\begin{document}
\noappendicestocpagenum
\addappheadtotoc
\begin{appendix}\label{ch:appendices}

	\begin{identity}[]

	\end{identity}

	\begin{identity}
		\begin{align*}
			(a+b)^3 - a^3 - b^3 &= 3ab(a+b)\\
			(a+b)^5 - a^5 - b^5 &= 5ab(a+b)(a^2+ab+b^2)\\
			(a+b)^7 - a^7 - b^7 &= 7ab(a+b)(a^2+ab+b^2)^2
		\end{align*}
	\end{identity}

	\begin{identity}[]\label{thm:binomial-theorem}

	\end{identity}

	\begin{identity} \label{thm:binom}

	\end{identity}

	\begin{identity}

	\end{identity}

	\begin{identity}[Sum of Powers of Consecutive Integers]\label{id:sumofpowers}
		Let $n$ be a positive integer. Then,
			\begin{enumerate}
				\item $\displaystyle\sum\limits_{i=1}^{n} i = \frac{n(n+1)}{2}$,
				\item $\displaystyle\sum\limits_{i=1}^{n} i^2 = \frac{n(n+1)(2n+1)}{6}$,
				\item $\displaystyle\sum\limits_{i=1}^{n} i^3 = \left(\frac{n(n+1)}{2}\right)^2$,
				\item $\displaystyle\sum\limits_{i=1}^{n} i^4 = \frac{n(n+1)(2n+1)(3n^2+3n-1)}{30}$.
			\end{enumerate}
	\end{identity}

	\begin{identity}[]\label{id:sumofdif}

	\end{identity}

	\begin{proof}

	\end{proof}


	\begin{identity}[y]\label{id:fibbr}

	\end{identity}



	\begin{identity}[]\label{id:foursqr}

	\end{identity}


	\begin{identity}[]\label{id:lebesgue}

	\end{identity}

	\begin{identity}[]\label{id:euleraida}

	\end{identity}

	\begin{identity}[]

	\end{identity}

\end{appendix}

\end{document}